pcuic/theories/PCUICArities.v
@@ -86,7 +86,7 @@ Proof.
           apply context_relation_app in convctx; auto.
           constructor; pcuic.
           eapply context_relation_app in convctx as [_ convctx].
-          unshelve eapply (context_relation_impl _ convctx).
+          unshelve eapply (context_relation_impl convctx).
           simpl; firstorder. destruct X. constructor; auto.
           eapply conv_conv_ctx; eauto.
           eapply context_relation_app_inv. constructor; pcuic.
@@ -98,13 +98,7 @@ Proof.
           eapply context_relation_app_inv. constructor; pcuic.
           constructor; pcuic. constructor; pcuic. now symmetry.
           apply context_relation_refl. intros.
-          destruct x as [na'' [b'|] ty']; constructor; reflexivity.
-          constructor; pcuic.
-          eapply conv_conv_ctx; eauto.
-          eapply context_relation_app_inv. constructor; pcuic.
-          constructor; pcuic. constructor; pcuic. now symmetry.
-          apply context_relation_refl. intros.
-          destruct x as [? [?|] ?]; constructor; reflexivity.
+          destruct x as [na'' [b''|] ty']; constructor; reflexivity.
           eapply conv_conv_ctx; eauto.
           eapply context_relation_app_inv. constructor; pcuic.
           constructor; pcuic. constructor; pcuic. now symmetry.
